fv/lean/Ragu/Circuits/Point/Spec.lean
@@ -10,8 +10,6 @@ structure Point (F : Type) where
   y : F
 deriving ProvableStruct
 
-
-
 /--
   NOTE: supports only short Weierstrass curves with a = 0
 
@@ -26,11 +24,13 @@ def Point.isOnCurve (point : Point (F p)) (curveParams : CurveParams (F p)) : Pr
 def CurveParams.noOrderTwoPoints (curveParams : CurveParams (F p)) : Prop :=
   (∀ point : Spec.Point (F p), (point.isOnCurve curveParams) → point.y ≠ 0)
 
-def Point.double (point : Point (F p)) : Point (F p) :=
-  -- TODO: a / 0 is defined to be 0 for fields, this is not a precise spec
+def Point.double (point : Point (F p)) : Option (Point (F p)) :=
+  -- a / 0 is defined to be 0 for fields, therefore to make the spec precise
+  -- we return None if point.y is zero
+  if point.y = 0 then none else
   let lambda := (3 * point.x^2) / (2 * point.y)
   let x2 := lambda^2 - 2*point.x
-  {
+  some {
     x := x2,
     y := lambda * (point.x - x2) - point.y
   }
@@ -47,10 +47,15 @@ open Spec
 
 lemma double_preserves_membership (point : Point (F p)) (curveParams: CurveParams (F p))
     (h_membership: point.isOnCurve curveParams) (h_order : curveParams.noOrderTwoPoints) :
-    point.double.isOnCurve curveParams := by
+    match point.double with
+    | none =>
+      -- this is impossible: since we assume that the curve does not have points of order two,
+      -- every affine point has an affine double
+      False
+    | some double => double.isOnCurve curveParams := by
   simp only [CurveParams.noOrderTwoPoints] at h_order
   specialize h_order point h_membership
-  simp only [Point.isOnCurve, Point.double]
+  simp only [Point.double, if_neg h_order, Point.isOnCurve]
   simp only [Point.isOnCurve] at h_membership
   have h2 : (2 : F p) ≠ 0 := NeZero.ne 2
   have h2y : (2 : F p) * point.y ≠ 0 := mul_ne_zero h2 h_order
